git/cruhland/lean4-axiomatic/Lean4Axiomatic/Natural/Impl/Derived.lean
@@ -1,4 +1,3 @@
 import Lean4Axiomatic.Natural.Impl.Derived.Addition
-import Lean4Axiomatic.Natural.Impl.Derived.Core
 import Lean4Axiomatic.Natural.Impl.Derived.Multiplication
 import Lean4Axiomatic.Natural.Impl.Derived.Order
